

$$T(n) = \begin{cases} c_1, & n=0 \\ c_2 + T(n-1), & n>0 \end{cases}$$

-1 הליכה

$$\begin{aligned} T(n) &= c_2 + T(n-1) = c_2 + (c_2 + T(n-2)) \\ &= 2c_2 + T(n-2) = 2c_2 + (c_2 + T(n-3)) = \\ &= 3c_2 + T(n-3) = \dots \end{aligned}$$

$$= i \cdot c_2 + T(n-i) \Rightarrow$$

כאשר $n-i=0$ נקבל $n=i$

$$n-i=0$$

$$n=i$$

$$T(n) = n \cdot c_2 + T(0) = n \cdot c_2 + c_1 = O(n)$$

$$T(n) = \begin{cases} c_1, & n=1 \\ c_2 + 2T(n/2), & n>1 \end{cases}$$

-2 הליכה

$$\begin{aligned} T(n) &= c_2 + 2T(n/2) = c_2 + 2(c_2 + 2T(n/4)) = \\ &= 3c_2 + 4T(n/4) = 3c_2 + 4(c_2 + 2T(n/8)) = \\ &= 7c_2 + 8T(n/8) = \dots \end{aligned}$$

$$= c_2 \cdot \sum_{k=0}^{i-1} 2^k + 2^i T(n/2^i)$$

$$i = \log n \quad n = 2^i \quad \text{כאשר } n/2^i = 1$$

$$T(n) = c_2 \cdot \sum_{k=0}^{\log n - 1} 2^k + n \cdot T(1) = c_2 \cdot (n-1) + n \cdot c_1 = O(n)$$

$$\text{סדרה מסוג } S = \sum_{n=N_1}^{N_2} q^n = a_1 \left(\frac{q^{N_1} - q^{N_2+1}}{1-q} \right) \cdot \sum_{k=0}^{\log n - 1} 2^k = 1 \left(\frac{2^0 - 2^{\log n}}{1-2} \right) = (n-1)$$

$$\textcircled{1} \quad T(n) = T(n-1) + \log n =$$

$$= T(n-2) + \log(n-1) + \log n =$$

$$= T(n-3) + \log(n-2) + \log(n-1) + \log n =$$

$$\vdots$$

$$= T(n-k) + \log(n-k+1) + \dots + \log(n-1) + \log n$$

$$n=k \Leftrightarrow n-k=0 \quad \text{פס 0-1 פס 2N נוסף נוסף}$$

$$T(n) = T(0) + \sum_{k=1}^n \log k = 1 + \log(n!) = \Theta(n \log n)$$

$$\textcircled{2} \quad T(n) = 3T(n/3) + 1 = 3(3T(n/3^2) + 1) + 1$$

$$= 9T(n/9) + 1 + 3 = 9(3T(n/3^3) + 1) + 1 + 3$$

$$= 27T(n/27) + 1 + 3 + 9$$

$$\vdots$$

$$= 3^k T(n/3^k) + \underbrace{\sum_{i=0}^{k-1} 3^i}$$

$$\frac{3^0 - 3^{\log_3 n}}{1-3} = \frac{n-1}{2}$$

נוסף נוסף

$$n/3^k = 1$$

$$n = 3^k$$

$$k = \log_3 n$$

$$T(n) = 3^{\log_3 n} T(1) + \frac{n-1}{2} = n + 1 + \frac{n-1}{2} = O(n)$$

$$\begin{aligned}
 \textcircled{3} \quad T(n) &= 3T\left(\frac{n}{3}\right) + n = 3\left(3T\left(\frac{n}{3^2}\right) + \frac{n}{3}\right) + n \\
 &= 9T\left(\frac{n}{9}\right) + 2n = 9\left(3T\left(\frac{n}{3^3}\right) + \frac{n}{3^2}\right) + 2n \\
 &= 27T\left(\frac{n}{27}\right) + 3n \\
 &\quad \vdots \\
 &= 3^k T\left(\frac{n}{3^k}\right) + kn
 \end{aligned}$$

$$k = \log_3 n \Leftarrow \frac{n}{3^k} = 1 \quad \text{1000 1030}$$

$$T(n) = 3^{\log_3 n} + T(1) + \log n \cdot n = n + 1 + n \log n = O(n \log n)$$

$$\log_a b = \frac{\log_c b}{\log_c a} \quad : \text{օժտություն}$$

$$T(n) = 9T(n/3) + n$$

$$a=9, b=3, f(n)=n, n^{\log_3 9} = n^2$$

$$T(n) = \Theta(n^2) \Leftarrow \text{המקרה הכללי} \quad n = O(n^{2-\epsilon})$$

$$T(n) = 5T(n/5) + n$$

$$a=5, b=5, f(n)=n, n^{\log_5 5} = n$$

$$T(n) = \Theta(n \log n) \Leftarrow f(n) = \Theta(n) \quad 2 \text{ מקרים}$$

$$T(n) = 8T(n/2) + n^3$$

$$a=8, b=2, f(n)=n^3, n^{\log_2 8} = n^3$$

$$T(n) = \Theta(n^3 \log n) \Leftarrow 2 \text{ מקרים}$$

$$T(n) = T(n/2) + \Theta(1)$$

$$a=1, b=2, f(n) = \Theta(1), n^{\log_2 1} = n^0 = 1$$

$$T(n) = \Theta(\log n) \Leftarrow 2 \text{ מקרים}$$

$$T(n) = 5T(n/4) + n^2$$

$$a=5, b=4, f(n)=n^2, n^{\log_4 5} = n^{1.1...}$$

$$T(n) = \Theta(n^2) \Leftarrow 1 > C > \frac{5}{16} \quad \Leftarrow \left(\frac{5}{4}\right)^2 < C \cdot n^2 \quad \Leftarrow 3 \text{ מקרים}$$